Updates.

FOL/NV/PredSub/All/Rec/PredSubAllRecFresh.lean
@@ -1,4 +1,6 @@
 import FOL.NV.PredSub.All.Rec.PredSubAllRecOption
+import FOL.NV.Alpha
+
 
 namespace FOL
 
@@ -9,224 +11,15 @@ open Formula
 
 def predVarFreeVarSet
   (τ : PredName → ℕ → Option (List VarName × Formula)) :=
-  fun (p, n) =>
-  match τ p n with
-  | none => {}
-  | some (zs, H) => H.freeVarSet \ zs.toFinset
-
-def subPredFresh
-  (c : Char)
-  (τ : PredName → ℕ → Option (List VarName × Formula)) :
-  Formula → Formula
-  | pred_const_ X xs => pred_const_ X xs
-  | pred_var_ X xs =>
-      let opt := τ X xs.length
+    fun (p, n) =>
+      let opt := τ p n
       if h : Option.isSome opt
       then
         let val := Option.get opt h
         let zs := val.fst
         let H := val.snd
-        if xs.length = zs.length
-        then subFresh (Function.updateListITE id zs xs) c H
-        else pred_var_ X xs
-      else pred_var_ X xs
-  | eq_ x y => eq_ x y
-  | true_ => true_
-  | false_ => false_
-  | not_ phi =>
-    have : length phi < length (not_ phi) := by simp only [Formula.length]; simp
-    not_ (subPredFresh c τ phi)
-  | imp_ phi psi =>
-      have : length phi < length (imp_ phi psi) := by simp only [Formula.length]; apply Nat.lt_add_right; simp;
-      have : length psi < length (imp_ phi psi) := by simp only [Formula.length]; simp;
-      imp_ (subPredFresh c τ phi) (subPredFresh c τ psi)
-  | and_ phi psi =>
-      have : length phi < length (and_ phi psi) := by simp only [Formula.length]; apply Nat.lt_add_right; simp;
-      have : length psi < length (and_ phi psi) := by simp only [Formula.length]; simp;
-      and_ (subPredFresh c τ phi) (subPredFresh c τ psi)
-  | or_ phi psi =>
-      have : length phi < length (or_ phi psi) := by simp only [Formula.length]; apply Nat.lt_add_right; simp;
-      have : length psi < length (or_ phi psi) := by simp only [Formula.length]; simp;
-      or_ (subPredFresh c τ phi) (subPredFresh c τ psi)
-  | iff_ phi psi =>
-      have : length phi < length (iff_ phi psi) := by simp only [Formula.length]; apply Nat.lt_add_right; simp;
-      have : length psi < length (iff_ phi psi) := by simp only [Formula.length]; simp;
-      iff_ (subPredFresh c τ phi) (subPredFresh c τ psi)
-  | forall_ x phi =>
-      have : length (subFresh (Function.updateITE id x (if x ∈ Finset.biUnion (predVarSet phi) (predVarFreeVarSet τ) then fresh x c (Finset.biUnion (predVarSet phi) (predVarFreeVarSet τ)) else x)) c phi) < length (forall_ x phi) := by simp only [Formula.length]; simp only [sub_formula_length_same]; simp;
-      let vs : Finset VarName := Finset.biUnion phi.predVarSet (predVarFreeVarSet τ)
-      let x' : VarName :=
-        if x ∈ vs
-        then fresh x c vs
-        else x
-      forall_ x' (subPredFresh c τ (subFresh (Function.updateITE id x x') c phi))
-  | exists_ x phi =>
-      have : length (subFresh
-      (Function.updateITE id x
-        (if x ∈ Finset.biUnion (predVarSet phi) (predVarFreeVarSet τ) then
-          fresh x c (Finset.biUnion (predVarSet phi) (predVarFreeVarSet τ) ∪ freeVarSet phi \ {x})
-        else x))
-      c phi) <
-  length (exists_ x phi) := by simp only [Formula.length]; simp only [sub_formula_length_same]; simp;
-      let vs : Finset VarName := Finset.biUnion phi.predVarSet (predVarFreeVarSet τ)
-      let x' : VarName :=
-        if x ∈ vs
-        then fresh x c (vs ∪ (phi.freeVarSet \ {x}))
-        else x
-      exists_ x' (subPredFresh c τ (subFresh (Function.updateITE id x x') c phi))
-  | def_ X xs => def_ X xs
-  termination_by subPredFresh c τ F => F.length
-
-
-example
-  (D : Type)
-  (I : Interpretation D)
-  (V V' : VarAssignment D)
-  (E : Env)
-  (σ : VarName → VarName)
-  (c : Char)
-  (τ : PredName → ℕ → Option (List VarName × Formula))
-  (F : Formula) :
-  --(h1 : ∀ (x : VarName), x ∈ Finset.biUnion (predVarSet F) (predVarFreeVarSet τ) → V' x = V x) :
-  Holds D
-    ⟨
-      I.nonempty,
-      I.pred_const_,
-      fun (X : PredName) (ds : List D) =>
-      let opt := τ X ds.length
-      if h : Option.isSome opt
-      then
-        let val := Option.get opt h
-        let zs := val.fst
-        let H := val.snd
-        if ds.length = zs.length
-        then Holds D I (Function.updateListITE V' zs ds) E H
-        else I.pred_var_ X ds
-      else I.pred_var_ X ds
-    ⟩
-    V E F ↔ Holds D I V E (subPredFresh c τ F) :=
-  by
-  induction F generalizing V
-  case pred_const_ X xs =>
-    unfold subPredFresh
-    simp only [Holds]
-  case pred_var_ X xs =>
-    --simp only [predVarSet] at h1
-    --simp at h1
-
-    unfold subPredFresh
-    simp only [Holds]
-    simp
-    split_ifs
-    case _ c1 c2 =>
-      let opt := τ X xs.length
-      let val := Option.get opt c1
-      let zs := val.fst
-      let H := val.snd
-      obtain s1 := substitution_fun_theorem' D I V E (Function.updateListITE id zs xs) c H
-      simp only [Function.updateListITE_comp] at s1
-      simp at s1
-      simp only [s1]
-      clear s1
-
-      apply Holds_coincide_Var
-      intro v a1
-      by_cases c3 : v ∈ zs
-      · apply Function.updateListITE_mem_eq_len V' V v zs (List.map V xs) c3
-        simp
-        simp only [← c2]
-      · simp only [Function.updateListITE_not_mem V v zs (List.map V xs) c3]
-        simp only [Function.updateListITE_not_mem V' v zs (List.map V xs) c3]
-        --apply h1
-        sorry
-    case _ c1 c2 =>
-      simp only [Holds]
-    case _ c1 =>
-      simp only [Holds]
-
-  case forall_ x phi phi_ih =>
-    --simp only [predVarSet] at h1
-
-    unfold subPredFresh
-    simp only [Holds]
-    apply forall_congr'
-    intro d
-
-    set pred_var_' := (fun X ds =>
-      let opt := τ X (List.length ds);
-      if h : Option.isSome opt = true
-      then
-        let val := Option.get opt h;
-        let zs := val.fst;
-        let H := val.snd;
-        if List.length ds = List.length zs
-        then Holds D I (Function.updateListITE V' zs ds) E H
-        else Interpretation.pred_var_ I X ds
-      else Interpretation.pred_var_ I X ds)
-
-    set I' := ({ nonempty := (_ : Nonempty D), pred_const_ := I.pred_const_, pred_var_ := pred_var_' } : Interpretation D)
-
-    obtain s1 := fresh_not_mem x c (Finset.biUnion (predVarSet phi) (predVarFreeVarSet τ))
-
-    generalize (fresh x c (Finset.biUnion (predVarSet phi) (predVarFreeVarSet τ))) = x' at *
-
-    split_ifs
-    case _ c1 =>
-      obtain s2 := substitution_fun_theorem D I
-      simp only [phi_ih]
-      sorry
-    case _ c1 =>
-      simp only [Function.updateITE_id]
-      simp only [SubId]
-      apply phi_ih
-/-
-      intro z a1
-      simp only [Function.updateITE]
-      split_ifs
-      case _ c2 =>
-        subst c2
-        contradiction
-      case _ c2 =>
-        exact h1 z a1
--/
-  all_goals sorry;
-
---------------------------------------------------
-
-def subPredCapturedAux
-  (binders : Finset VarName)
-  (τ : PredName → ℕ → Option (List VarName × Formula)) :
-  Formula → Finset VarName
-  | pred_const_ _ _ => ∅
-  | pred_var_ X xs =>
-      let opt := τ X xs.length
-      if h : Option.isSome opt
-      then
-        let val := Option.get opt h
-        let zs := val.fst
-        let H := val.snd
-        if xs.length = zs.length
-        then binders ∩ (H.freeVarSet \ zs.toFinset)
-        else ∅
-      else ∅
-  | eq_ _ _ => ∅
-  | true_ => ∅
-  | false_ => ∅
-  | not_ phi => subPredCapturedAux binders τ phi
-  | imp_ phi psi => subPredCapturedAux binders τ phi ∪ subPredCapturedAux binders τ psi
-  | and_ phi psi => subPredCapturedAux binders τ phi ∪ subPredCapturedAux binders τ psi
-  | or_ phi psi => subPredCapturedAux binders τ phi ∪ subPredCapturedAux binders τ psi
-  | iff_ phi psi => subPredCapturedAux binders τ phi ∪ subPredCapturedAux binders τ psi
-  | forall_ x phi => subPredCapturedAux (binders ∪ {x}) τ phi
-  | exists_ x phi => subPredCapturedAux (binders ∪ {x}) τ phi
-  | def_ _ _ => ∅
-
-
-def subPredCaptured
-  (τ : PredName → ℕ → Option (List VarName × Formula))
-  (F : Formula) :
-  Finset VarName :=
-  subPredCapturedAux ∅ τ F
+        H.freeVarSet \ zs.toFinset
+      else {}
 
 
 def subPredAlphaAux
@@ -241,7 +34,7 @@ def subPredAlphaAux
   | true_ => true_
   | false_ => false_
   | not_ phi =>
-    not_ (subPredAlphaAux c τ α binders phi)
+      not_ (subPredAlphaAux c τ α binders phi)
   | imp_ phi psi =>
       imp_
       (subPredAlphaAux c τ α binders phi)
@@ -259,13 +52,92 @@ def subPredAlphaAux
       (subPredAlphaAux c τ α binders phi)
       (subPredAlphaAux c τ α binders psi)
   | forall_ x phi =>
-      let free := phi.freeVarSet \ (binders ∪ {x})
-      let replaced_free := (replacePredFun c τ phi).freeVarSet
-      let captured := subPredCapturedAux (binders ∪ {x}) τ phi
-      let x' :=
-        if captured = ∅
-        then x
-        else fresh x c (replaced_free ∪ free)
+      let vs : Finset VarName := Finset.biUnion phi.predVarSet (predVarFreeVarSet τ)
+      let x' : VarName :=
+        if x ∈ vs
+        then fresh x c vs
+        else x
       forall_ x' (subPredAlphaAux c τ (Function.updateITE α x x') (binders ∪ {x'}) phi)
-  | exists_ x phi => sorry
+  | exists_ x phi =>
+      let vs : Finset VarName := Finset.biUnion phi.predVarSet (predVarFreeVarSet τ)
+      let x' : VarName :=
+        if x ∈ vs
+        then fresh x c vs
+        else x
+      exists_ x' (subPredAlphaAux c τ (Function.updateITE α x x') (binders ∪ {x'}) phi)
   | def_ X xs => def_ X (xs.map α)
+
+
+example
+  (D : Type)
+  (I : Interpretation D)
+  (V : VarAssignment D)
+  (E : Env)
+  (c : Char)
+  (τ : PredName → ℕ → Option (List VarName × Formula))
+  (α : VarName → VarName)
+  (binders : Finset VarName)
+  (F : Formula)
+  (h1 : ∀ (x : VarName), x ∈ binders → x ∉ (Finset.biUnion F.predVarSet (predVarFreeVarSet τ)))
+  :
+  admitsPredFunAux τ binders (subPredAlphaAux c τ α binders F) :=
+  by
+  induction F generalizing α binders
+  case pred_var_ X xs =>
+    simp only [predVarSet] at h1
+    simp at h1
+
+    simp only [subPredAlphaAux]
+    simp only [admitsPredFunAux]
+    split_ifs
+    case _ c1 c2 =>
+      simp at c1
+
+      apply Finset.eq_empty_of_forall_not_mem
+      simp
+      intro x a1 a2
+      specialize h1 x a1
+      simp only [predVarFreeVarSet] at h1
+      simp only [c1] at h1
+      simp at h1
+      exact h1 a2
+  case forall_ x phi phi_ih =>
+    simp only [predVarSet] at h1
+
+    simp only [subPredAlphaAux]
+    simp only [admitsPredFunAux]
+    split_ifs
+    case pos c1 =>
+      obtain s1 := fresh_not_mem x c (Finset.biUnion (predVarSet phi) (predVarFreeVarSet τ))
+
+      generalize (fresh x c (Finset.biUnion (predVarSet phi) (predVarFreeVarSet τ))) = x' at *
+
+      have s2 : ¬ x' = x
+      intro contra
+      subst contra
+      apply s1
+      exact c1
+
+      apply phi_ih
+      intro x_1 a1
+      simp at a1
+      cases a1
+      case _ c2 =>
+        apply h1
+        exact c2
+      case _ c2 =>
+        subst c2
+        exact s1
+    case neg c1 =>
+      apply phi_ih
+      intro x_1 a1
+      simp at a1
+      cases a1
+      case _ c2 =>
+        apply h1
+        exact c2
+      case _ c2 =>
+        subst c2
+        exact c1
+  all_goals
+    sorry
